updating minor local changes

HybridVerifVecs/FVs/AMV_Example.thy
@@ -15,19 +15,42 @@ theory AMV_Example
 
 begin
 
+definition "no_modfs X i \<equiv> \<forall>k. (\<lambda>s. s$i = k) \<le> |X] (\<lambda>s. s$i = k)"
+
+lemma no_modfs_inv:
+  "no_modfs X i \<Longrightarrow> (\<lambda>s. Q (s$i)) \<le> |X] (\<lambda>s. Q (s$i))"
+  unfolding fbox_def no_modfs_def by (clarsimp simp: le_fun_def)
 
 subsubsection \<open> Type of variables \<close>
 
-(* continuous variables *)
+(* Continuous Variables
+  AMV's position vector: (x, y)
+  AMV's velocity vector: (vx, vy)
+  AMV's acceleration vector: (ax, ay)
+  angle of AMV's velocity vector with horizontal: phi \<in> [-\<pi>,\<pi>]
+  speed of AMV's: speed
+  time: t
+  [Therefore:
+    s^2 = vx^2 + vy^2
+    (vx, vy) = (speed * cos phi, speed * sgn phi * sin phi)  *)
 abbreviation "amv_cstrs \<equiv> {''x'', ''y'', ''vx'', ''vy'', ''ax'', ''ay'', 
   ''phi'', ''speed'', ''t''}"
 
-(* discrete variables *)
-abbreviation "amv_dstrs \<equiv> {''sSP'', ''hSP'', ''fx'', ''fy'', ''mode''}"
+(* Discrete Variables 
+  Speed Set Point: sSP
+  Heading Set Point: hSP (radians)
+  Longitudinal Acceleration Force: fl (colinear with velocity vector)
+  Radial Acceleration Force: fr (perpendicular to fl)
+  AMV's mode: mode
+    operator control          - OCM
+    main operating mode       - MOM
+    high caution mode         - HCM
+    collision avoidance mode  - CAM *)
+abbreviation "amv_dstrs \<equiv> {''sSP'', ''hSP'', ''fl'', ''fr'', ''mode''}" 
 
 (* all variables *)
 abbreviation "amv_strs \<equiv> {''x'', ''y'', ''vx'', ''vy'', ''ax'', ''ay'', 
-  ''phi'', ''speed'', ''t'', ''sSP'', ''hSP'', ''fx'', ''fy'', ''mode''}"
+  ''phi'', ''speed'', ''t'', ''sSP'', ''hSP'', ''fl'', ''fr'', ''mode''}"
 
 (* type of variables *)
 typedef AMV = amv_strs
@@ -37,7 +60,7 @@ typedef AMV = amv_strs
 notation to_var ("\<downharpoonright>\<^sub>V")
 
 abbreviation "amv_terms \<equiv> {\<downharpoonright>\<^sub>V''x'', \<downharpoonright>\<^sub>V''y'', \<downharpoonright>\<^sub>V''vx'', \<downharpoonright>\<^sub>V''vy'', \<downharpoonright>\<^sub>V''ax'', \<downharpoonright>\<^sub>V''ay'', 
-  \<downharpoonright>\<^sub>V''phi'', \<downharpoonright>\<^sub>V''speed'', \<downharpoonright>\<^sub>V''t'', \<downharpoonright>\<^sub>V''sSP'', \<downharpoonright>\<^sub>V''hSP'', \<downharpoonright>\<^sub>V''fx'', \<downharpoonright>\<^sub>V''fy'', \<downharpoonright>\<^sub>V''mode''}"
+  \<downharpoonright>\<^sub>V''phi'', \<downharpoonright>\<^sub>V''speed'', \<downharpoonright>\<^sub>V''t'', \<downharpoonright>\<^sub>V''sSP'', \<downharpoonright>\<^sub>V''hSP'', \<downharpoonright>\<^sub>V''fl'', \<downharpoonright>\<^sub>V''fr'', \<downharpoonright>\<^sub>V''mode''}"
 
 lemma number_of_program_vars: "CARD(AMV) = 14"
   using type_definition.card type_definition_AMV by fastforce
@@ -58,19 +81,19 @@ lemma AMV_univ: "(UNIV::AMV set) = amv_terms"
 
 lemma AMV_exhaust: "x = \<downharpoonright>\<^sub>V''x'' \<or> x = \<downharpoonright>\<^sub>V''y'' \<or> x = \<downharpoonright>\<^sub>V''vx'' \<or> x = \<downharpoonright>\<^sub>V''vy'' 
   \<or> x = \<downharpoonright>\<^sub>V''ax'' \<or> x = \<downharpoonright>\<^sub>V''ay'' \<or> x = \<downharpoonright>\<^sub>V''phi'' \<or> x = \<downharpoonright>\<^sub>V''speed'' 
-  \<or> x = \<downharpoonright>\<^sub>V''t'' \<or> x=\<downharpoonright>\<^sub>V''sSP'' \<or> x=\<downharpoonright>\<^sub>V''hSP'' \<or> x=\<downharpoonright>\<^sub>V''fx'' \<or> x=\<downharpoonright>\<^sub>V''fy'' \<or> x=\<downharpoonright>\<^sub>V''mode''"
+  \<or> x = \<downharpoonright>\<^sub>V''t'' \<or> x=\<downharpoonright>\<^sub>V''sSP'' \<or> x=\<downharpoonright>\<^sub>V''hSP'' \<or> x=\<downharpoonright>\<^sub>V''fl'' \<or> x=\<downharpoonright>\<^sub>V''fr'' \<or> x=\<downharpoonright>\<^sub>V''mode''"
   using AMV_univ by auto
 
 lemma AMV_sum:
   fixes f :: "AMV \<Rightarrow> ('a::banach)"
   shows "(\<Sum>i\<in>UNIV. f i) = f (\<downharpoonright>\<^sub>V''x'') + f (\<downharpoonright>\<^sub>V''y'') + f (\<downharpoonright>\<^sub>V''vx'') + f (\<downharpoonright>\<^sub>V''vy'') 
   + f (\<downharpoonright>\<^sub>V''ax'') + f (\<downharpoonright>\<^sub>V''ay'') + f (\<downharpoonright>\<^sub>V''phi'') + f (\<downharpoonright>\<^sub>V''speed'') + f (\<downharpoonright>\<^sub>V''t'')
-  + f (\<downharpoonright>\<^sub>V''sSP'') + f (\<downharpoonright>\<^sub>V''hSP'') + f (\<downharpoonright>\<^sub>V''fx'') + f (\<downharpoonright>\<^sub>V''fy'') + f (\<downharpoonright>\<^sub>V''mode'')"
+  + f (\<downharpoonright>\<^sub>V''sSP'') + f (\<downharpoonright>\<^sub>V''hSP'') + f (\<downharpoonright>\<^sub>V''fl'') + f (\<downharpoonright>\<^sub>V''fr'') + f (\<downharpoonright>\<^sub>V''mode'')"
   unfolding AMV_univ by (simp add: to_var_inject)
 
 lemma AMV_induct: "P (\<downharpoonright>\<^sub>V''x'') \<Longrightarrow> P (\<downharpoonright>\<^sub>V''y'') \<Longrightarrow> P (\<downharpoonright>\<^sub>V''vx'') \<Longrightarrow> P (\<downharpoonright>\<^sub>V''vy'') 
   \<Longrightarrow> P (\<downharpoonright>\<^sub>V''ax'') \<Longrightarrow> P (\<downharpoonright>\<^sub>V''ay'') \<Longrightarrow> P (\<downharpoonright>\<^sub>V''phi'') \<Longrightarrow> P (\<downharpoonright>\<^sub>V''speed'') \<Longrightarrow> P (\<downharpoonright>\<^sub>V''t'')
-  \<Longrightarrow> P (\<downharpoonright>\<^sub>V''sSP'') \<Longrightarrow> P (\<downharpoonright>\<^sub>V''hSP'') \<Longrightarrow> P (\<downharpoonright>\<^sub>V''fx'') \<Longrightarrow> P (\<downharpoonright>\<^sub>V''fy'') \<Longrightarrow> P (\<downharpoonright>\<^sub>V''mode'')
+  \<Longrightarrow> P (\<downharpoonright>\<^sub>V''sSP'') \<Longrightarrow> P (\<downharpoonright>\<^sub>V''hSP'') \<Longrightarrow> P (\<downharpoonright>\<^sub>V''fl'') \<Longrightarrow> P (\<downharpoonright>\<^sub>V''fr'') \<Longrightarrow> P (\<downharpoonright>\<^sub>V''mode'')
   \<Longrightarrow> \<forall>i. P i"
   using AMV_exhaust by metis
 
@@ -79,7 +102,7 @@ lemma AMV_eq:
   s1\<restriction>\<^sub>V''vy'' = s2\<restriction>\<^sub>V''vy'' \<and> s1\<restriction>\<^sub>V''ax'' = s2\<restriction>\<^sub>V''ax'' \<and> s1\<restriction>\<^sub>V''ay'' = s2\<restriction>\<^sub>V''ay'' \<and>
   s1\<restriction>\<^sub>V''phi'' = s2\<restriction>\<^sub>V''phi'' \<and> s1\<restriction>\<^sub>V''speed'' = s2\<restriction>\<^sub>V''speed'' \<and> s1\<restriction>\<^sub>V''t'' = s2\<restriction>\<^sub>V''t'' \<and>
   s1\<restriction>\<^sub>V''sSP'' = s2\<restriction>\<^sub>V''sSP'' \<and> s1\<restriction>\<^sub>V''hSP'' = s2\<restriction>\<^sub>V''hSP'' \<and> 
-  s1\<restriction>\<^sub>V''fx'' = s2\<restriction>\<^sub>V''fx'' \<and> s1\<restriction>\<^sub>V''fy'' = s2\<restriction>\<^sub>V''fy'' \<and> s1\<restriction>\<^sub>V''mode'' = s2\<restriction>\<^sub>V''mode'')"
+  s1\<restriction>\<^sub>V''fl'' = s2\<restriction>\<^sub>V''fl'' \<and> s1\<restriction>\<^sub>V''fr'' = s2\<restriction>\<^sub>V''fr'' \<and> s1\<restriction>\<^sub>V''mode'' = s2\<restriction>\<^sub>V''mode'')"
   apply(clarsimp simp: vec_eq_iff, rule iffI, force)
   by (rule AMV_induct, auto)
 
@@ -131,29 +154,40 @@ abbreviation amv_guard :: "real \<Rightarrow> real \<Rightarrow> real^AMV \<Righ
     0 \<le> s\<restriction>\<^sub>V''speed'' \<and> s\<restriction>\<^sub>V''speed'' \<le> S"
 
 (* abbreviation "Dynamics \<equiv> \<^bold>c:t := 0 ;; ODE" *)
-abbreviation "amv_dyn \<epsilon> S  s \<equiv> (\<downharpoonright>\<^sub>V''t'' ::= (\<lambda>s. 0)) ; (x\<acute>= f & (G \<epsilon> S))"
+abbreviation "amv_dyn \<epsilon> S \<equiv> (\<downharpoonright>\<^sub>V''t'' ::= (\<lambda>s. 0)) ; (x\<acute>= f & (G \<epsilon> S))"
 
 
 subsubsection \<open> Formalisation of discrete control \<close>
 
 locale AMV =
   fixes \<epsilon> :: real \<comment> \<open> max. time for ODE \<close>
-    and S :: real \<comment> \<open> max. speed of AMV \<close>
-    and H :: real \<comment> \<open> max. speed of AMV \<close>
-    and HCM :: real \<comment> \<open> modes \<close>
-    and MOM :: real
-    and OCM :: real
+    and "e\<^sub>\<Phi>" :: real \<comment> \<open> angle hysteresis \<close>
+    and "s\<^sub>\<epsilon>" :: real \<comment> \<open> speed setpoint limiter \<close>
+    and "\<Phi>\<^sub>\<epsilon>" :: real \<comment> \<open> angle setpoint limiter\<close>
+    and flmax :: real \<comment> \<open> maximum force capable by motor \<close>
+    and frmax :: real \<comment> \<open> maximum rotational force capable by motor \<close>
+    and "k\<^sub>l" :: real \<comment> \<open> proportionality controller constant for longitudinal force \<close>
+    and "k\<^sub>r" :: real \<comment> \<open> proportionality controller constant for radial force \<close>
+    and m :: real \<comment> \<open> mass of the AMV \<close>
+    and S :: real \<comment> \<open> max. (controlling) speed of AMV \<close> (* as opposed to that by laws of physics *)
+    and H :: real \<comment> \<open> min. (controlling) speed of AMV \<close>
+    and HCM :: real \<comment> \<open> high caution mode \<close>
+    and MOM :: real \<comment> \<open> main operating mode \<close>
+    and OCM :: real \<comment> \<open> operator control mode \<close>
     and wp :: "real^2" \<comment> \<open> waypoint's position  \<close>
     and Obs :: "(real^2) set" \<comment> \<open> set of obstacles \<close>
   assumes "Obs = {(\<chi> i::2. (1::real))}"
     and "HCM = 1"
     and "MOM = 2"
     and "OCM = 3"
+    and mass: "m > 0"
+    and longF: "flmax > 0"
+    and rotF: "frmax > 0"
 begin
 
 (* abbreviation "angOfVec \<equiv> vangle \<^bold>[[0::real,100]\<^bold>]"
    abbreviation "steerToWP \<equiv> rh := angOfVec(nextWP - &\<^bold>c:p)" *)
-abbreviation "steerToWP \<equiv> (\<downharpoonright>\<^sub>V''t'' ::= (\<lambda>s. vangle (\<chi> i. if i=1 then 0 else 100) (wp - pos s)))"
+abbreviation "steerToWP \<equiv> (\<downharpoonright>\<^sub>V''hSP'' ::= (\<lambda>s. vangle (\<chi> i. if i=1 then 0 else 100) (wp - pos s)))"
 
 lemma "vector [0,100] = (\<chi> i::2. if i=1 then (0::real) else 100)"
   apply(simp add: vec_eq_iff vector_def)
@@ -167,18 +201,131 @@ lemma "vector [0,100] = (\<chi> i::2. if i=1 then (0::real) else 100)"
              steerToWP ;; 
              if (\<exists> o. o \<in> obsReg \<and> \<parallel>&\<^bold>c:p - \<guillemotleft>o\<guillemotright>\<parallel> \<le> 7.5) then mode := HCM ;; rs := 0.1 fi
           )" *)
-abbreviation "LRE s \<equiv> if s\<restriction>\<^sub>V''mode'' = HCM then ((\<downharpoonright>\<^sub>V''sSP'' ::= (\<lambda>s. H)) ; steerToWP) s else {s}"
 
+abbreviation "nearObj k s \<equiv> \<exists>ob \<in> Obs. \<parallel>pos s - ob\<parallel> \<le> k"
+abbreviation "onCollCourse k s \<equiv> \<exists>ob \<in> Obs. \<parallel>pos s - ob\<parallel> \<le> k \<and> vangle (ob - pos s) (vel s) < e\<^sub>\<Phi>"
+
+abbreviation "LRE k \<equiv> 
+  IF (\<lambda>s. s\<restriction>\<^sub>V''mode'' = HCM) THEN 
+    (\<downharpoonright>\<^sub>V''sSP'' ::= (\<lambda>s. H)) ; steerToWP
+  ELSE (IF (\<lambda>s. s\<restriction>\<^sub>V''mode'' = MOM) THEN 
+    (\<downharpoonright>\<^sub>V''sSP'' ::= (\<lambda>s. S)); steerToWP;
+    (IF nearObj k THEN 
+      (\<downharpoonright>\<^sub>V''mode'' ::= (\<lambda>s. HCM));(\<downharpoonright>\<^sub>V''sSP'' ::= (\<lambda>s. H)) 
+    ELSE skip)
+  ELSE skip)"
+
+(*
+abbreviation "AP \<equiv> 
+  if \<parallel>rs - &\<^bold>c:s\<parallel> > s\<^sub>\<epsilon>
+    then ft := sgn(rs - &\<^bold>c:s)*min(kp\<^sub>g\<^sub>v * \<parallel>rs - &\<^bold>c:s\<parallel>) f\<^sub>m\<^sub>a\<^sub>x
+    else ft := 0 fi ;; 
+  if \<parallel>rh - &\<^bold>c:\<phi>\<parallel> > \<phi>\<^sub>\<epsilon>
+    then fl := sgn(rh - &\<^bold>c:\<phi>)*min(kp\<^sub>g\<^sub>r * \<parallel>rh - &\<^bold>c:\<phi>\<parallel>) f\<^sub>m\<^sub>a\<^sub>x
+    else fl := 0 fi ;;
+  f := fl *\<^sub>R \<^bold>[[cos(&\<^bold>c:\<phi>), sin(&\<^bold>c:\<phi>)]\<^bold>] 
+     + ft *\<^sub>R \<^bold>[[sin(&\<^bold>c:\<phi>), cos(&\<^bold>c:\<phi>)]\<^bold>] ;;
+  \<^bold>c:a := f /\<^sub>R m"
+*)
+abbreviation "AP \<equiv> 
+  (IF (\<lambda>s. \<bar>s\<restriction>\<^sub>V''sSP'' - s\<restriction>\<^sub>V''speed''\<bar> > s\<^sub>\<epsilon>) THEN 
+    (\<downharpoonright>\<^sub>V''fl'' ::= (\<lambda>s. sgn (s\<restriction>\<^sub>V''sSP'' - s\<restriction>\<^sub>V''speed'') * (min (k\<^sub>l * \<bar>s\<restriction>\<^sub>V''sSP'' - s\<restriction>\<^sub>V''speed''\<bar>) flmax))) 
+  ELSE 
+    (\<downharpoonright>\<^sub>V''fl'' ::= (\<lambda>s. 0)));
+  (IF (\<lambda>s. \<bar>s\<restriction>\<^sub>V''hSP'' - s\<restriction>\<^sub>V''phi''\<bar> > \<Phi>\<^sub>\<epsilon>) THEN 
+    (\<downharpoonright>\<^sub>V''fr'' ::= (\<lambda>s. sgn (s\<restriction>\<^sub>V''hSP'' - s\<restriction>\<^sub>V''phi'') * (min (k\<^sub>r * \<bar>s\<restriction>\<^sub>V''hSP'' - s\<restriction>\<^sub>V''phi''\<bar>) frmax))) 
+  ELSE 
+    (\<downharpoonright>\<^sub>V''fr'' ::= (\<lambda>s. 0)));
+  (\<downharpoonright>\<^sub>V''ax'' ::= (\<lambda>s. (s\<restriction>\<^sub>V''fl'' * cos (s\<restriction>\<^sub>V''phi'') + s\<restriction>\<^sub>V''fr'' * sin (s\<restriction>\<^sub>V''phi''))/m));
+  (\<downharpoonright>\<^sub>V''ay'' ::= (\<lambda>s. (s\<restriction>\<^sub>V''fl'' * sin (s\<restriction>\<^sub>V''phi'') + s\<restriction>\<^sub>V''fr'' * cos (s\<restriction>\<^sub>V''phi''))/m))"
+
+
+(* abbreviation "AUV \<equiv> (LRE ;; AP ;; Dynamics)\<^sup>\<star>" *)
+abbreviation "AUV \<equiv> (LRE 7.5; AP; amv_dyn \<epsilon> S)"
+
+lemma LRE_no_modfs:
+  shows LRE_no_modfs_t: "no_modfs (LRE 7.5) (\<downharpoonright>\<^sub>V''t'')"
+    and LRE_no_modfs_x: "no_modfs (LRE 7.5) (\<downharpoonright>\<^sub>V''x'')"
+    and LRE_no_modfs_y: "no_modfs (LRE 7.5) (\<downharpoonright>\<^sub>V''y'')"
+    and LRE_no_modfs_vx: "no_modfs (LRE 7.5) (\<downharpoonright>\<^sub>V''vx'')"
+    and LRE_no_modfs_vy: "no_modfs (LRE 7.5) (\<downharpoonright>\<^sub>V''vy'')"
+    and LRE_no_modfs_ax: "no_modfs (LRE 7.5) (\<downharpoonright>\<^sub>V''ax'')"
+    and LRE_no_modfs_ay: "no_modfs (LRE 7.5) (\<downharpoonright>\<^sub>V''ay'')"
+    and LRE_no_modfs_speed: "no_modfs (LRE 7.5) (\<downharpoonright>\<^sub>V''speed'')"
+    and LRE_no_modfs_phi: "no_modfs (LRE 7.5) (\<downharpoonright>\<^sub>V''phi'')"
+  unfolding no_modfs_def by (auto simp: to_var_inject)
+
+lemma AP_no_modfs:
+  shows AP_no_modfs_t: "no_modfs AP (\<downharpoonright>\<^sub>V''t'')"
+    and AP_no_modfs_x: "no_modfs AP (\<downharpoonright>\<^sub>V''x'')"
+    and AP_no_modfs_y: "no_modfs AP (\<downharpoonright>\<^sub>V''y'')"
+    and AP_no_modfs_vx: "no_modfs AP (\<downharpoonright>\<^sub>V''vx'')"
+    and AP_no_modfs_vy: "no_modfs AP (\<downharpoonright>\<^sub>V''vy'')"
+    and AP_no_modfs_speed: "no_modfs AP (\<downharpoonright>\<^sub>V''speed'')"
+    and AP_no_modfs_phi: "no_modfs AP (\<downharpoonright>\<^sub>V''phi'')"
+  unfolding no_modfs_def by (auto simp: to_var_inject)
+
+lemma amv_dyn_no_modfs_sSP: "no_modfs (amv_dyn a b) (\<downharpoonright>\<^sub>V''sSP'')"
+  unfolding no_modfs_def apply (rule allI)
+  apply(rule_tac R="\<lambda>s. s\<restriction>\<^sub>V''sSP'' = k" in hoare_kcomp, simp_all add: to_var_inject)
+  by (auto intro!: diff_invariant_rules poly_derivatives simp: to_var_inject)
+
+lemma amv_dyn_no_modfs_hSP: "no_modfs (amv_dyn a b) (\<downharpoonright>\<^sub>V''hSP'')"
+  unfolding no_modfs_def apply (rule allI)
+  apply(rule_tac R="\<lambda>s. s\<restriction>\<^sub>V''hSP'' = k" in hoare_kcomp, simp_all add: to_var_inject)
+  by (auto intro!: diff_invariant_rules poly_derivatives simp: to_var_inject)
+
+lemma amv_dyn_no_modfs_fr: "no_modfs (amv_dyn a b) (\<downharpoonright>\<^sub>V''fr'')"
+  unfolding no_modfs_def apply (rule allI)
+  apply(rule_tac R="\<lambda>s. s\<restriction>\<^sub>V''fr'' = k" in hoare_kcomp, simp_all add: to_var_inject)
+  by (auto intro!: diff_invariant_rules poly_derivatives simp: to_var_inject)
+
+lemma amv_dyn_no_modfs_fl: "no_modfs (amv_dyn a b) (\<downharpoonright>\<^sub>V''fl'')"
+  unfolding no_modfs_def apply (rule allI)
+  apply(rule_tac R="\<lambda>s. s\<restriction>\<^sub>V''fl'' = k" in hoare_kcomp, simp_all add: to_var_inject)
+  by (auto intro!: diff_invariant_rules poly_derivatives simp: to_var_inject)
+
+lemma "G \<epsilon> S \<le> |LRE 7.5] G \<epsilon> S"
+  by (auto simp: to_var_inject vec_eq_iff)
+
+lemma "(\<lambda>s. s\<restriction>\<^sub>V''t'' \<ge> 0) \<le> |x\<acute>= f & (G \<epsilon> S)] (\<lambda>s. s\<restriction>\<^sub>V''t'' \<ge> 0)"
+  apply(simp, rule_tac \<nu>'="\<lambda>s. 0" and \<mu>'="\<lambda>s. 1" in diff_invariant_leq_rule)
+  apply(auto intro!: poly_derivatives)
+  by (erule_tac x="\<downharpoonright>\<^sub>V''t''" in allE, simp add: to_var_inject)
+
+lemma "(\<lambda>s. s\<restriction>\<^sub>V''speed'' = \<parallel>vel s\<parallel>) \<le> |x\<acute>= f & (G \<epsilon> S)] (\<lambda>s. s\<restriction>\<^sub>V''speed'' = \<parallel>vel s\<parallel>)"
+  apply(rule diff_weak_rule, clarsimp)
+  apply(drule sym, simp, simp add: norm_vec_def L2_set_def)
+  unfolding UNIV_2 by auto
+
+lemma "(\<lambda>s. s\<restriction>\<^sub>V''sSP'' = s\<restriction>\<^sub>V''speed'' \<and> s\<restriction>\<^sub>V''hSP'' = s\<restriction>\<^sub>V''phi'') \<le> |AP] (\<lambda>s. acc s = 0)"
+  by (auto simp: to_var_inject vec_eq_iff)
+
+lemma "(\<lambda>s. s\<restriction>\<^sub>V''speed'' \<in> {s\<restriction>\<^sub>V''sSP'' - s\<^sub>\<epsilon> .. s\<restriction>\<^sub>V''sSP'' + s\<^sub>\<epsilon>} \<and> s\<restriction>\<^sub>V''hSP'' = s\<restriction>\<^sub>V''phi'') \<le> |AP] (\<lambda>s. acc s = 0)"
+  apply (auto simp: to_var_inject vec_eq_iff)
+  done
+
+lemma "(\<lambda>s. s\<restriction>\<^sub>V''sSP'' < s\<restriction>\<^sub>V''speed'' - s\<^sub>\<epsilon> \<and> s\<restriction>\<^sub>V''hSP'' = s\<restriction>\<^sub>V''phi'') \<le> |AP] (\<lambda>s. \<parallel>acc s\<parallel> > 0)"
+  using sin_zero_abs_cos_one mass longF rotF
+  apply (auto simp: to_var_inject vec_eq_iff)
+  using exhaust_2 apply fastforce
+
+
+
+lemma "(\<lambda>s. acc s \<bullet> vel s = (\<parallel>acc s\<parallel>) * (\<parallel>vel s\<parallel>)) \<le> |amv_dyn a b] (\<lambda>s. acc s \<bullet> vel s = (\<parallel>acc s\<parallel>) * (\<parallel>vel s\<parallel>))"
+  apply(rule_tac R="\<lambda>s. acc s \<bullet> vel s = (\<parallel>acc s\<parallel>) * (\<parallel>vel s\<parallel>)" in hoare_kcomp)
+  apply(simp add: le_fun_def)
+   apply(simp add: inner_vec_def norm_vec_def L2_set_def )
+
+  oops
+
+
+thm to_str_induct to_str_inject to_str_inverse
+thm to_var_induct to_var_inject to_var_inverse
 
 end
 
-
-(* vangle *)
-term vangle
-
 no_notation f_amv ("f")
         and amv_guard ("G")
-
-
 
 end
